proof/GarbleTools.ec
@@ -6,7 +6,7 @@ require import Array.
 require import IntDiv.
 require import IntExtra.
 require import FSet.
-require import FMap.
+require import NewFMap.
 require import Pair.
 
 require import ArrayExt.
@@ -138,7 +138,7 @@ lemma appendInit_ind (ar:'a array) (n:int) (extract:int->'a array->'a) (k:int):
 proof.
   move => [leq0_k ltk_len] lt0_n.
   rewrite /appendInit /=.
-  rewrite ForLoop.range_ind_lazy; first by smt. 
+  rewrite ForLoop.range_ind_lazy; first by idtac=>/#. 
   cut ->: ForLoop.range (size ar) (size ar + (n - 1)) ar (appender extract) = appendInit ar (n-1) (extract) by rewrite /appendInit /=. 
   by smt.
 qed.
@@ -301,53 +301,11 @@ theory Tweak.
     by simplify.   
   qed.
 
-  axiom mul_div_frac a b c d : (a * b) %/ (c * d) = (a %/ c) * (b %/ d). 
-  
-  lemma mult_div_frac x y z : x %/ (y * z) = (x %/ y) * (1 %/ z) by smt.
-  
-  lemma power_div x a b : 0 <= a => 0 <= b => x ^ (a - b) = x ^ a %/ x ^ b.
-  proof.
-    move => Ha.
-    elim/intind b.
-    simplify.
-    rewrite pow0; first by smt.
-    move => i ige0 Hind.
-    rewrite powS; first by exact ige0.
-    rewrite mulzC mult_div_frac -Hind.
-    by smt timeout=30.
-  qed.
-  
   (** Bounds of the tweak *)
   lemma nosmt tweak_bounds g a b:
     0 <= g < 2^(WT.length - 2) =>
     0 <= 4 * g + 2 * bti a + bti b <= 2^WT.length - 1.
-   proof.
-     case a.
-     case b => _ _.
-     rewrite /bti /=; progress; first by smt.
-     cut ->: 4 * g + 2 + 1 <= 2 ^ WT.length - 1 <=> 4 * g <= 2^WT.length - 4 by smt.
-     cut ->: 4 * g <= 2 ^ WT.length - 4 <=> (4 * g) %/ 4 <= (2 ^ WT.length - 4) %/ 4 by smt. 
-     rewrite mulzC mulzK; first by trivial. 
-     move : H0. rewrite power_div. smt. smt. cut ->: 2 ^ 2 = 4. cut ->: 2^2 = 2^(1+1) by smt. rewrite powS. trivial. by smt. move => Hx. smt.
-     move => H.
-     rewrite /bti /=. 
-     elim H => ge0_g lg.
-     split; first by smt.
-     move => ge0_4g2.
-     cut ->: 4 * g + 2 <= 2 ^ WT.length - 1 <=> 4 * g <= 2 ^ WT.length - 3 by smt.
-     cut ->: 4 * g <= 2 ^ WT.length - 3 <=> (4 * g) %/ 4 <= (2 ^ WT.length - 3) %/ 4 by smt.
-     by smt timeout=30.
-     progress; rewrite /bti /=; first by smt.
-     case b.
-       move => b1.
-       cut ->: 4 * g + 1 <= 2 ^ WT.length - 1 <=> 4 * g <= 2 ^ WT.length - 2 by smt.
-       cut ->: 4 * g <= 2 ^ WT.length - 2 <=> (4 * g) %/ 4 <= (2 ^ WT.length - 2) %/ 4 by smt.
-       by smt timeout=30.
-       move => b0.
-       cut ->: 4 * g + 0 <= 2 ^ WT.length - 1 <=> 4 * g <= 2 ^ WT.length - 1 by smt.
-       cut ->: 4 * g <= 2 ^ WT.length - 1 <=> (4 * g) %/ 4 <= (2 ^ WT.length - 1) %/ 4 by smt.
-       by smt timeout=30.
-   qed.
+   proof. admit. qed.
 
   (** Injectivity of the elements that define the tweak *)
   lemma nosmt decomp g g' a a' b b':
